interpreter example

Freigen/CompM/Examples/Nondet/Basic.lean
@@ -5,6 +5,11 @@ import Freigen.ITree.Basic
 
 namespace Freigen.CompM.Examples.Nondet
 
+/-!
+Basic examples: two diverging computations, one deterministic one not + sample
+evaluations and determinisim proofs.
+-/
+
 def scaryLoop : Nondet Unit := do
   while true do
     let x ← Nondet.rand
@@ -22,36 +27,34 @@ example : approxWith Int.ofNat scaryLoopDet 20 = [0, 0, 0, 0, 0, 0, 0] := by rfl
 
 def Deterministic {α} (t : Nondet α) : Prop := SamePrints Eq t t
 
--- theorem scaryLoopDet_deterministic : Deterministic scaryLoopDet := by
---   apply SamePrints.bind
---   · apply SamePrints.loop
---     grind [SamePrints.bind, SamePrints.rand, SamePrints.print, SamePrints.ret]
---   · simp [SamePrints.ret]
-
-theorem scaryLoopDet_deterministic : Deterministic scaryLoopDet := by
+open SamePrints in
+example : Deterministic scaryLoopDet := by
   apply SamePrints.bind
   · apply SamePrints.loop_coind (I := Eq) (RR := Eq) rfl
     rintro ⟨⟩ _ rfl
-    conv =>
-      congr
-      · skip
-      · skip
-      · rw [loop_def]
-      · rw [loop_def]
+    apply Step.loop
     simp only [↓reduceIte, Int.sub_self, bind_pure_comp, bind_assoc, bind_map_left]
-    apply SamePrints.Step.silent
-    · apply SamePrints.Silent.rand
-    · apply SamePrints.Silent.rand
+    apply Step.rand_rand
     intros
-    apply SamePrints.Steps.step (SamePrints.Step.print _)
-    apply SamePrints.Steps.step
-    apply SamePrints.Step.silent
-    · apply SamePrints.Silent.tick
-    · apply SamePrints.Silent.tick
-    intros
-    apply SamePrints.Steps.recur
-    simp [SamePrints.LoopPair]
+    apply Steps.print
+    apply Steps.tick_tick
+    apply Steps.recur
+    simp [LoopPair]
   · simp [SamePrints.ret]
+
+example : ¬Deterministic scaryLoop := by
+  unfold scaryLoop
+  simp only [forIn]
+  rw [loop_def]
+  simp only [↓reduceIte, bind_pure_comp, bind_assoc, bind_map_left, map_bind, id_map']
+  apply SamePrints.not_rand 0 1
+  apply SamePrints.not_print
+  omega
+
+/-!
+More involved (weak) bisimulation: desynchronized infinite loops shown to
+produce the same traces.
+-/
 
 def printAllInts : Nondet Unit := do
   let mut curr := 0
@@ -69,32 +72,98 @@ def printAllIntsBy2 : Nondet Unit := do
 #eval approxWith Int.ofNat printAllInts 20
 #eval approxWith Int.ofNat printAllIntsBy2 20
 
+open SamePrints in
 example : SamePrints Eq printAllInts printAllIntsBy2 := by
   apply SamePrints.bind
   · apply SamePrints.loop_coind Eq (RR := Eq) (by simp)
     rintro s _ rfl
-    conv =>
-      congr
-      · skip
-      · skip
-      · rw [loop_def]
-        simp only [↓reduceIte, bind_pure_comp, map_pure, bind_map_left]
-        rw [loop_def]
-      · rw [loop_def]
+    apply Step.loop
     simp only [↓reduceIte, bind_pure_comp, map_pure, bind_map_left, bind_assoc]
-    apply SamePrints.Step.print
-    apply SamePrints.Steps.step
-    apply SamePrints.Step.silentL
-    · apply SamePrints.Silent.tick
-    intros
-    apply SamePrints.Step.print
-    apply SamePrints.Steps.step
-    apply SamePrints.Step.silent
-    · apply SamePrints.Silent.tick
-    · apply SamePrints.Silent.tick
-    intros
-    apply SamePrints.Steps.recur
-    grind [SamePrints.LoopPair]
+    apply Step.print
+    apply Steps.tick_left
+    apply Step.loop_left
+    simp only [bind_map_left]
+    apply Step.print
+    apply Steps.tick_tick
+    apply Steps.recur
+    grind [LoopPair]
+  · simp [SamePrints.ret]
+
+/-!
+A bytecode interpreter for a simple register machine – just write the interpreter like we
+would in Rust, then talk about what it does.
+-/
+
+abbrev Register := Fin 10
+
+inductive Op : Type
+| const (n : ℤ) (r : Register) -- r <- n
+| rand (r : Register) -- r <- rand
+| sub (r1 r2 r3 : Register) -- r3 <- r1 - r2
+| print (r : Register) -- print r
+| goto (r : Register) -- goto (pc + r)
+| done
+
+abbrev Program := Array Op
+
+structure State where
+  regs : Register → ℤ
+  pc : Nat
+
+def State.init : State where
+  regs := fun _ => 0
+  pc := 0
+
+def State.getReg (s : State) (r : Register) : ℤ := s.regs r
+def State.setReg (s : State) (r : Register) (v : ℤ) : State :=
+  { s with regs := fun r' => if r' = r then v else s.regs r' }
+def State.addPC (s : State) (n : ℤ) : State := { s with pc := (Int.ofNat s.pc + n).toNat }
+
+def Op.denote (op : Op) (s : State) : Nondet $ Option State := do
+  match op with
+  | .const n r => pure $ (s.setReg r n).addPC 1
+  | .rand r => (some ∘ State.setReg (s.addPC 1) r) <$> Nondet.rand
+  | .sub r1 r2 r3 => pure $ (s.setReg r3 (s.getReg r1 - s.getReg r2)).addPC 1
+  | .print r => (Nondet.print $ s.getReg r) *> pure (some $ s.addPC 1)
+  | .goto r => pure $ some (s.addPC (s.getReg r))
+  | .done => pure none
+
+def Program.denote (p : Program) : Nondet Unit := do
+  let mut state := some State.init
+  while let some s := state do
+    let op := p.getD s.pc Op.done
+    state ← op.denote s
+
+def exampleProgram : Program := #[
+  .rand 0,
+  .sub 0 0 0,
+  .print 0,
+  .const (-5) 0,
+  .goto 0
+]
+
+#eval approxWith Int.ofNat exampleProgram.denote 200
+
+open SamePrints in
+example : Deterministic exampleProgram.denote := by
+  apply SamePrints.bind (RR := Eq)
+  simp [forIn]
+  apply SamePrints.loop_coind (I := fun s₁ s₂ =>
+    (∃reg₁, s₁ = some ⟨reg₁, 0⟩) ∧
+    (∃reg₂, s₂ = some ⟨reg₂, 0⟩)
+  ) (RR := Eq)
+  · simp [State.init]
+  · rintro s₁ s₂ ⟨⟨r₁, rfl⟩, ⟨r₂, rfl⟩⟩
+    simp [exampleProgram, Op.denote]
+    repeat (first
+      | apply Steps.recur; grind only [LoopPair]
+      | apply Steps.tick_tick
+      | apply Steps.print
+      | apply Step.rand_rand; intros
+      | apply Steps.loop
+      | apply Step.loop
+      | simp [State.getReg, State.setReg, State.addPC, seqRight_eq_bind, State.addPC]
+    )
   · simp [SamePrints.ret]
 
 end Freigen.CompM.Examples.Nondet
